---
title: "Partial Derivatives"
subtitle: "Session 02"  
author: 
  - "Alejandro Ucan"
date: '`r Sys.Date()`'
output:
  xaringan::moon_reader:
    css: xaringan-themer.css
    nature:
      slideNumberFormat: "%current%"
      highlightStyle: github
      highlightLines: true
      ratio: 16:9
      countIncrementalSlides: true
---

```{r setup, include=FALSE}
options(htmltools.dir.version = FALSE)
knitr::opts_chunk$set(
  fig.width=9, fig.height=3.5, fig.retina=3,
  out.width = "100%",
  cache = FALSE,
  echo = FALSE,
  message = FALSE, 
  warning = FALSE,
  hiline = TRUE
)
```

```{r xaringan-themer, include=FALSE, warning=FALSE}
library(xaringanthemer)
style_duo_accent(
  primary_color = "#000080",
  secondary_color = "#f2f3f4",
  inverse_header_color = "#00147e"
)
```

```{r xaringan-editable, echo=FALSE}
xaringanExtra::use_editable(expires = 1)
xaringanExtra::use_scribble()
```
# Goals of the Session

  * We will introduce the concept of partial derivatives. <br/><br/>
  * We will apply the general rules of partial derivatives. <br/><br/>

---
# Motivation

The **heat index** ( $I$ ) measures the combined effects of temperature and humidity. $I$ measures the sensation of air temperature when the temperature is $T$ and the relative humidity is $H.$

![SensaciÃ³n Termica](SensacionTermica.png)

--


What is the rate of change of $I$ when we change $T$ at the point $(96,70)$?

---
# Partial Derivative

> __Definition:__ Given a function $f:\mathbb{R}^n\to \mathbb{R},$ the partial derivative with respect to the variable $x_j,$ denoted by $f_{x_j}=\frac{\partial f}{\partial x_j},$ is defined as the limit $$\lim_{h\to 0} \frac{f(x_1,\cdots,x_j+h,x_{j+1},\cdots, x_n)-f(x_1,\cdots,x_j,x_{j+1},\cdots, x_n)}{h}.$$
--

#### Example 1: 

Compute the partial derivative with respect to $x$ of the function $f(x,y)=3xy.$

--
$$f_x(x,y)=\lim_{h\to 0}\frac{3(x+h)y-3xy}{h}=\lim_{h\to 0}\frac{3(x+h-x)y}{h}=\lim_{h\to 0}\frac{3yh}{h}=3y.$$

---
#### Example 3:

Compute the partial derivative with respect to $y$ of the function $f(x,y,z)=xy-zx+4y.$

--
<br/><br/>
$$f_y(x,y,z)=\lim_{h\to 0}\frac{x(y+h)-zx+4(y+h)-(xy-zx+4y)}{h}=\lim_{h\to 0}\frac{xh+4h}{h}=x+4.$$
--
<br/><br/>
respect to $z$?

--
<br/><br/>
$$f_z(x,y,z)=\lim_{h\to 0}\frac{xy-(z+h)x+4y-(xy-zx+4y)}{h}=\lim_{h\to 0}\frac{hx}{h}=x.$$

---
## How to Partially Derive?

> To partially derive a function with respect to a variable, we just derive the function assuming that the other variables are constants.
--

#### Example 4:

Compute the partial derivatives $f_x,\,f_y$ and $f_z$ for the next functions: <br/><br/>


* $f(x,y,z)=\frac{\sin(x)}{z}+x\cos(y)$
* $f(x,y,z)=z^2e^{x+y}$
* $f(x,y,z)=x\ln(z)+y\sqrt{x}.$

---
# Geometric Interpretation of Partial Derivatives

Hereby we present the graph of the function $f(x,y)=x^2+xy+y^3$ at the point $(1,1).$

<iframe src="https://www.geogebra.org/calculator/aemfszpg?embed" width="1200" height="400" allowfullscreen style="border: 1px solid #e4e4e4;border-radius: 4px;" frameborder="0"></iframe>

---
# Modelling with Partial Derivatives:

> The Argentine inflation (in 2019) is given by the function $h(x,y)=e^{x+y}\sqrt{4-3x^2-2y^2},$ where $h$ is measured in percentage, and $(x,y)$ represents a point in the city. If we observe at the point $(1,1)$, what is the rate of change of inflation when we move in the vertical direction? And in the horizontal direction?

--

$$\frac{\partial f}{\partial x}=-e^{x + y} \frac{-4 + 3 x + 3 x^2 + 2 y^2}{\sqrt{4 - 3 x^2 - 2 y^2}}$$

$$\frac{\partial f}{\partial y}=-e^{x + y} \frac{3 x^2 + 2 (-2 + y + y^2)}{\sqrt{4 - 3 x^2 - 2 y^2}}$$

---
# Implicit Partial Derivation

#### Example 5:

Assume that $x,y,z$ satisfy the following equation: $$x^2+y^2-z^2=0.$$ Compute $z_x$ and $z_y.$

--
<br/><br/>
We have that  $$\frac{\partial z}{\partial x}=\frac{x}{z}$$ $$\frac{\partial z}{\partial y}=\frac{y}{z}.$$

---
# Properties of Partial Derivatives

> __Theorem:__ Let $f,g:\mathbb{R}^n\to\mathbb{R}$ two function where $n=2,3.$ The following are valid:
<br/><br/>
  * $(f\pm g)_x=f_x\pm g_x.$ <br/><br/>
  * $(fg)_x = (f_x)g + f(g_x).$ <br/><br/>
  * If $g\neq 0,$ then $(f/g)_x =\frac{(f_x)g-f(g_x)}{g^2}.$

