---
title: "Chain Rule"
subtitle: "Session 04"  
author: 
  - "Alejandro Ucan"
date: '`r Sys.Date()`'
output:
  xaringan::moon_reader:
    css: xaringan-themer.css
    nature:
      slideNumberFormat: "%current%"
      highlightStyle: github
      highlightLines: true
      ratio: 16:9
      countIncrementalSlides: true
---

```{r setup, include=FALSE}
options(htmltools.dir.version = FALSE)
knitr::opts_chunk$set(
  fig.width=9, fig.height=3.5, fig.retina=3,
  out.width = "100%",
  cache = FALSE,
  echo = FALSE,
  message = FALSE, 
  warning = FALSE,
  hiline = TRUE
)
```

```{r xaringan-themer, include=FALSE, warning=FALSE}
library(xaringanthemer)
style_duo_accent(
  primary_color = "#000080",
  secondary_color = "#f2f3f4",
  inverse_header_color = "#00147e"
)
```

```{r xaringan-editable, echo=FALSE}
xaringanExtra::use_editable(expires = 1)
xaringanExtra::use_scribble()
```
# Goals for the Session:

  * Introduce the concept of change of variables. <br/><br/>
  * Define the chain rule. <br/><br/>
  * Apply the chain rule. <br/><br/>

---
# Motivation:

> Consider the function $W(T,v)=13.12+0.62T -11.37v^{0.16}+0.39Tv^{0.16}$ that measures the body's thermal sensation where $T$ is the temperature and $v$ is the wind speed. <br/><br/>
But, both $T$ and $v$ depend on the position of the city where we are: $$T(x,y)=17+3xy$$ $$v(x,y)=-x^2+y^2$$
<br/><br/>
Using a substitution we can express the Thermal sensation in terms of position doing: $$W(T(x,y),v(x,y))$$

---
# Change of variables

> **Definition:** A change of variables for a function $f:\mathbb{R}^n\to \mathbb{R}$ is a collection of $n-$functions $g_1,\cdots,g_n:\mathbb{R}^m\to\mathbb{R}$ such that $$f(g_1(x_1,\cdots, x_m),g_2(x_1,\cdots, x_m),\cdots,g_n(x_1,\cdots, x_m)).$$

--

#### Example 1:

Consider the function $f(x,y)=xy$ and the change of variable $$x(u,v,w)=u+v+w\quad y(u,v,w)=u-v+w.$$ Compute the function $f$ with its change of variable.

--

$$f(x(u,v,w),y(u,v,w))=(u+v+w)(u-v+w).$$

---

#### Example 2:

Consider the function $f(x,y)=\ln(x\cos(y^2))$ and the change of variable $$x(u,v)=\sin(uv)\quad y(u,v)=e^{uv}.$$ Compute the function $f$ with its change of variable.

--
$$f(x(u,v),y(u,v))=\ln(\sin(uv)\cos(e^{2uv}))$$
---
#### Example 3:

Consider the function $f(x,y,z)=\sqrt{x^2+y^2+z^2}$ and the change of variable $$x(u,v)=\sin(u) \quad y(u,v)=\cos(u)\quad z(u,v)=uv.$$ Compute the function $f$ with its change of variable.

--
$$ f(x(u,v),y(u,v),z(u,v))=\sqrt{u^2v^2 + 1}$$

---
# Chain Rule

> **Theorem:** Assume that $u:\mathbb{R}^n\to \mathbb{R}$ is a function of $n-$variables and $g_1,\cdots,g_n:\mathbb{R}^m\to\mathbb{R}$ are functions of $m-$variables. Then, the chain rule states that $$\frac{\partial u}{\partial x_j}=\frac{\partial u}{\partial u}\frac{\partial g_2}{\partial x_j}+ \frac{\partial u}{\partial g_2}\frac{\partial g_2}{\partial x_j}+\cdots +\frac{\partial u}{\partial u}\frac{\partial g_n}{\partial x_j}$$ for $j=1,\cdots,m.$

---
 # How it looks like that chain rule?
 
 ![Chain Rule](Regla_Cadena.jpg)

---

#### Example 1:

Compute the partial derivatives of the function $f(x,y)=xy$ with the change of variable $$x(u,v,w)=u+v+w\quad y(u,v,w)=u-v+w.$$

--
$$f_u(u,v,w)=(u-v+w)+(u+v+w)$$ $$f_v(u,v,w)=(u-v+w)-(u+v+w)$$
$$f_w(u,v,w)=(u-v+w)+(u+v+w)$$

---

#### Example 2:

Compute the partial derivatives of the function $f(x,y)=\ln(x\cos(y^2))$ with the change of variable $$x(u,v)=\sin(uv)\quad y(u,v)=e^{uv}.$$

--

$$ f_u(u,v)=\frac{1}{\sin(uv)}\cos(uv)v+\frac{-2e^{xy}\sin(e^{2uv})}{\sin(uv)\cos(e^{2uv})}ve^{uv}$$